examples/rv/rv32.v
@@ -1,34 +1,31 @@
-(*! Pipelined instantiation of the core !*)
+(*! Definition of a pipelined schedule !*)
 Require Import Koika.Frontend.
 Require Import RV.RVCore.
-Import RV32ICore.
 
 Definition rv_schedule : scheduler :=
   Writeback |> Execute |> StepMultiplier |> Decode |> WaitImem |> Fetch |> Imem |> Dmem |> UART_write |> Tick |> done.
 
-Definition circuits :=
-  compile_scheduler rv_rules rv_external rv_schedule.
+Module Package (C: Core).
+  Import C.
+  Existing Instance Show_reg_t.
+  Existing Instance Show_ext_fn_t.
+  Existing Instance FiniteType_reg_t.
 
-Instance Show_rf : Show (Rf.reg_t) :=
-  {| show '(Rf.rData v) := rv_register_name v |}.
+  Definition circuits :=
+    compile_scheduler rv_rules rv_external rv_schedule.
 
-Instance Show_scoreboard : Show (Scoreboard.reg_t) :=
-  {| show '(Scoreboard.Scores (Scoreboard.Rf.rData v)) := rv_register_name v |}.
+  Definition koika_package :=
+    {| koika_reg_types := R;
+       koika_reg_init := r;
+       koika_ext_fn_types := Sigma;
+       koika_rules := rv_rules;
+       koika_rule_external := rv_external;
+       koika_scheduler := rv_schedule;
+       koika_module_name := "rv32" |}.
 
-Definition koika_package :=
-  {| koika_reg_types := R;
-     koika_reg_init := r;
-     koika_ext_fn_types := Sigma;
-     koika_rules := rv_rules;
-     koika_rule_external := rv_external;
-     koika_scheduler := rv_schedule;
-     koika_module_name := "rv32" |}.
-
-Definition package :=
-  {| ip_koika := koika_package;
-     ip_sim := {| sp_ext_fn_names fn := show fn;
-                 sp_extfuns := None |};
-     ip_verilog := {| vp_ext_fn_specs := rv_ext_fn_specs |} |}.
-
-Definition prog := Interop.Backends.register package.
-Extraction "rv32.ml" prog.
+  Definition package :=
+    {| ip_koika := koika_package;
+       ip_sim := {| sp_ext_fn_names fn := show fn;
+                   sp_extfuns := None |};
+       ip_verilog := {| vp_ext_fn_specs := rv_ext_fn_specs |} |}.
+End Package.
