examples/rv/rv32e.v
@@ -1,0 +1,5 @@
+(*! Pipelined instantiation of an RV32E core !*)
+Require Import RV.RVCore RV.rv32.
+Module RV32EPackage := Package RV32E.
+Definition prog := Interop.Backends.register RV32EPackage.package.
+Extraction "rv32e.ml" prog.
